Continued with PPlusProperties and through SemAction inlining.

PPlusProperties.v
@@ -807,6 +807,956 @@ Proof.
   - econstructor 11; eauto.
 Qed.
 
+Inductive PSemAction_meth_collector (f : DefMethT) (o : RegsT) : RegsT -> RegsT -> MethsT -> MethsT -> Prop :=
+|NilCalls : PSemAction_meth_collector f o nil nil nil nil
+|ConsCalls reads1 reads2 reads upds1 upds2
+           upds calls1 calls2 calls calls'
+           calls'' argV retV:
+   PSemAction_meth_collector f o reads1 upds1 calls1 calls' ->
+   DisjKey upds1 upds2 ->
+   reads [=] reads1 ++ reads2 ->
+   upds [=] upds1 ++ upds2 ->
+   calls [=] calls1 ++ calls2 ->
+   calls'' [=] ((fst f, (existT _ (projT1 (snd f)) (argV, retV)))::calls') ->
+   PSemAction o (projT2 (snd f) type argV) reads2 upds2 calls2 retV ->
+   PSemAction_meth_collector f o reads upds calls calls''.
+
+Lemma Produce_action_from_collector (f : DefMethT) (o : RegsT) reads upds calls calls' call:
+  In call calls' ->
+  PSemAction_meth_collector f o reads upds calls calls' ->
+  exists reads1 reads2 upds1 upds2 calls1 calls2 calls'' argV retV,
+    DisjKey upds1 upds2 /\
+    upds [=] upds2++upds1 /\
+    calls [=] calls2++calls1 /\
+    reads [=] reads2 ++ reads1 /\
+    call = (fst f, (existT _ (projT1 (snd f)) (argV, retV))) /\
+    calls' [=] call::calls'' /\
+    PSemAction o (projT2 (snd f) type argV) reads2 upds2 calls2 retV /\
+    PSemAction_meth_collector f o reads1 upds1 calls1 calls''.
+Proof.
+  induction 2.
+  - contradiction.
+  - rewrite H5 in H.
+    destruct H.
+    + exists reads1, reads2, upds1, upds2, calls1, calls2, calls', argV, retV; subst.
+      repeat split; auto; (rewrite H2 || rewrite H3 || rewrite H4 || rewrite H5); subst; auto; apply Permutation_app_comm.
+    + specialize (IHPSemAction_meth_collector H); dest.
+      rewrite H8, H9, H10, H12 in *.
+      exists (reads2++x), x0, (upds2++x1), x2, (calls2++x3), x4, ((fst f, existT _ (projT1 (snd f)) (argV, retV))::x5), x6, x7.
+      repeat split; auto.
+      * intro; destruct (H7 k), (H1 k); rewrite map_app,in_app_iff in *; dest; firstorder fail.
+      (* * intro; destruct (H10 x8), (H2 x8); rewrite in_app_iff, DeM1 in *;[right|left; firstorder|right| right;assumption]; *)
+      (*     rewrite H13, in_app_iff, DeM1 in H20; firstorder. *)
+      * rewrite H3, <-app_assoc; apply Permutation_app_head, Permutation_app_comm.
+      * rewrite H4, <-app_assoc; apply Permutation_app_head, Permutation_app_comm.
+      * rewrite H2, <-app_assoc; apply Permutation_app_head, Permutation_app_comm.
+      * rewrite H5; apply perm_swap.
+      * econstructor.
+        -- apply H14.
+        -- assert (DisjKey x1 upds2).
+           ++ intro; destruct (H1 k);[rewrite map_app,in_app_iff,DeM1 in *; dest; left; assumption|right; assumption].
+           ++ apply H15.
+        (* -- intro; specialize (H2 x8). *)
+        (*    rewrite H13, in_app_iff, DeM1 in H2; destruct H2;[dest; left; assumption|right; apply H2]. *)
+        (* -- intro; specialize (H3 x8). *)
+        (*    rewrite H6, H7 in H3; repeat rewrite in_app_iff, DeM1 in H3; simpl in *; destruct H3;[left; intro; apply H3|right;rewrite in_app_iff, DeM1]; firstorder. *)
+        -- apply Permutation_app_comm.
+        -- apply Permutation_app_comm.
+        -- apply Permutation_app_comm.
+        -- reflexivity.
+        -- assumption.
+Qed.
+
+Lemma collector_perm_rewrite f o reads upds calls calls1':
+  PSemAction_meth_collector f o reads upds calls calls1' ->
+  forall calls2',
+    calls1' [=] calls2' ->
+    PSemAction_meth_collector f o reads upds calls calls2'.
+Proof.
+  induction 1; intros.
+  - apply Permutation_nil in H; subst.
+    constructor.
+  - rewrite H6 in H4.
+    econstructor; eauto.
+Qed.
+
+Global Instance collector_perm_rewrite' :
+  Proper (eq ==> eq ==> eq ==> eq ==> eq ==> (@Permutation MethT) ==> iff) (@PSemAction_meth_collector) | 10.
+Proof.
+  repeat red; intro; split; intros; subst; eauto using collector_perm_rewrite, Permutation_sym.
+Qed.
+
+Lemma collector_split (f : DefMethT) o calls1' calls2' :
+  forall  reads upds calls,
+  PSemAction_meth_collector f o reads upds calls (calls1'++calls2') ->
+  exists reads1 reads2 upds1 upds2 calls1 calls2,
+    reads [=] reads1 ++ reads2 /\
+    upds [=] upds1 ++ upds2 /\
+    calls [=] calls1 ++ calls2 /\
+    PSemAction_meth_collector f o reads1 upds1 calls1 calls1' /\
+    PSemAction_meth_collector f o reads2 upds2 calls2 calls2'.
+Proof.
+  induction calls1'; simpl; intros.
+  - exists nil, reads, nil, upds, nil, calls.
+    repeat split; auto.
+    constructor.
+  - specialize (Produce_action_from_collector _ (in_eq _ _) H) as TMP; dest.
+    apply Permutation_cons_inv in H5.
+    rewrite <- H5 in H7.
+    specialize (IHcalls1' _ _ _ H7) as TMP; dest.
+    exists (x0++x8), x9, (x2++x10), x11, (x4++x12), x13.
+    repeat split.
+    + rewrite H8, app_assoc in H3; assumption.
+    + rewrite H9, app_assoc in H1; assumption.
+    + rewrite H10, app_assoc in H2; assumption.
+    + econstructor.
+      * apply H11.
+      * rewrite H9 in H0; assert (DisjKey x10  x2);[intro; specialize (H0 k);
+                                                     rewrite map_app, in_app_iff in *;clear - H0; firstorder|apply H13].
+      (* * setoid_rewrite H9 in H1. *)
+      (*   assert (forall x, ~In x x12 \/ ~In x x4);[intro; specialize (H1 x14); rewrite in_app_iff in *; clear - H1; firstorder| apply H13]. *)
+      (* * intro; specialize (H2 x14); rewrite H4, H12 in H2. *)
+      (*   simpl in *; repeat rewrite in_app_iff in *. *)
+      (*   clear - H2; firstorder. *)
+      * apply Permutation_app_comm.
+      * apply Permutation_app_comm.
+      * apply Permutation_app_comm.
+      * rewrite H4; reflexivity.
+      * assumption.
+    + assumption.
+Qed.
+
+Lemma collector_correct_fst f o reads upds calls calls' call :
+  In call calls' ->
+  PSemAction_meth_collector f o reads upds calls calls' ->
+  fst call = fst f.
+Proof.
+  intros.
+  specialize (Produce_action_from_collector _ H H0) as TMP; dest.
+  destruct call; inv H5; simpl; reflexivity.
+Qed.
+
+Definition called_by (f : DefMethT) (call :MethT) : bool :=
+  (getBool (string_dec (fst f) (fst call))).
+
+Notation complement f := (fun x => negb (f x)).
+
+Definition called_execs (calls : MethsT) (exec : RuleOrMeth) : bool :=
+  match exec with
+  | Rle _ => false
+  | Meth f => existsb (methcmp f) calls
+  end.
+
+Lemma separate_calls_by_filter (A : Type) (l : list A) (f : A -> bool):
+  l [=] (filter f l) ++ (filter (complement f) l).
+Proof.
+  induction l; auto; simpl.
+  destruct (f a); simpl; rewrite IHl at 1;[reflexivity|apply Permutation_middle].
+Qed.
+
+Lemma reduce_called_execs_list execs c :
+  ~In (Meth c) execs ->
+  forall calls,
+    (filter (called_execs (c::calls)) execs) = (filter (called_execs calls) execs).
+Proof.
+  induction execs; intros; auto.
+  unfold called_execs, methcmp in *; destruct a; simpl in *.
+  - eapply IHexecs.
+    intro; apply H.
+    right; assumption.
+  - destruct MethT_dec; simpl.
+    + apply False_ind; apply H.
+      rewrite e; left; reflexivity.
+    + rewrite IHexecs;[reflexivity|].
+      intro; apply H; right; assumption.
+Qed.
+
+Corollary collector_called_by_filter_irrel f o calls' :
+  forall reads upds calls,
+  PSemAction_meth_collector f o reads upds calls calls' ->
+  (filter (called_by f) calls') = calls'.
+Proof.
+  induction calls'; intros; auto.
+  specialize (collector_correct_fst _ (in_eq _ _) H); intro.
+  unfold called_by; simpl; destruct string_dec;[simpl;fold (called_by f)|symmetry in H0; contradiction].
+  specialize (Produce_action_from_collector _ (in_eq _ _ ) H) as TMP; dest.
+  apply Permutation_cons_inv in H6.
+  rewrite <- H6 in H8.
+  erewrite IHcalls'; eauto.
+Qed.
+
+Corollary collector_complement_called_by_filter_nil f o calls' :
+  forall reads upds calls,
+    PSemAction_meth_collector f o reads upds calls calls' ->
+    (filter (complement (called_by f)) calls') = nil.
+Proof.
+  intros.
+  specialize (separate_calls_by_filter calls' (called_by f)) as parti.
+  rewrite (collector_called_by_filter_irrel H) in parti.
+  rewrite <- app_nil_r in parti at 1.
+  apply Permutation_app_inv_l in parti.
+  apply Permutation_nil in parti; assumption.
+Qed.
+
+Lemma collector_correct_snd f o reads upds calls calls' call :
+  In call calls' ->
+  PSemAction_meth_collector f o reads upds calls calls' ->
+  exists argV retV,
+    snd call = (existT _ (projT1 (snd f)) (argV, retV)).
+Proof.
+  intros.
+  specialize (Produce_action_from_collector _ H H0) as TMP; dest.
+  destruct call; inv H5; simpl; exists x6, x7; reflexivity.
+Qed.
+
+Lemma notIn_filter_nil (f : DefMethT) (calls : MethsT) :
+  ~In (fst f) (map fst calls) ->
+  filter (called_by f) calls = nil.
+Proof.
+  induction calls; auto; simpl.
+  intro; dest.
+  unfold called_by; destruct string_dec; simpl; auto.
+  apply False_ind, H; auto.
+Qed.
+
+Lemma notIn_complement_filter_irrel (f : DefMethT) (calls : MethsT) :
+  ~In (fst f) (map fst calls) ->
+  filter (complement (called_by f)) calls = calls.
+Proof.
+  induction calls; auto; simpl; intros.
+  unfold called_by in *; destruct string_dec; simpl in *;
+    [apply False_ind, H|rewrite IHcalls];auto.
+Qed.
+
+Lemma filter_complement_disj (A : Type) (dec : forall (a1 a2 : A), {a1=a2}+{a1<>a2}) (f : A -> bool) (l : list A) :
+  forall x, ~In x (filter f l) \/ ~In x (filter (complement f) l).
+Proof.
+  intros.
+  destruct (in_dec dec x (filter f l)).
+  - rewrite filter_In in i; dest.
+    right; intro.
+    rewrite filter_In in H1; dest.
+    rewrite H0 in H2; discriminate.
+  - left; assumption.
+Qed.
+
+Lemma PSemAction_NoDup_Key_Writes k o (a : ActionT type k) readRegs newRegs calls (fret : type k) :
+  PSemAction o a readRegs newRegs calls fret ->
+  NoDup (map fst newRegs).
+Proof.
+  induction 1;
+    eauto;[|
+           rewrite HANewRegs; simpl; econstructor; eauto; intro;
+           specialize (fst_produce_snd _ _ H0) as TMP; dest; specialize (HDisjRegs x);
+           contradiction| | |subst; econstructor];
+    rewrite HUNewRegs; rewrite map_app,NoDup_app_iff; repeat split; eauto;
+        repeat intro; specialize (HDisjRegs a0); firstorder.
+Qed.
+
+Corollary PSemAction_NoDup_Writes k o (a : ActionT type k) readRegs newRegs calls (fret : type k) :
+  PSemAction o a readRegs newRegs calls fret ->
+  NoDup newRegs.
+Proof.
+  intros; apply PSemAction_NoDup_Key_Writes in H; apply NoDup_map_inv in H; assumption.
+Qed.
+
+Lemma collector_NoDupRegs1 (f : DefMethT) o reads upds calls calls' :
+  PSemAction_meth_collector f o reads upds calls calls' ->
+  NoDup (map fst upds).
+Proof.
+  induction 1.
+  - constructor.
+  - rewrite H2, map_app, NoDup_app_iff.
+    specialize (PSemAction_NoDup_Key_Writes H5) as ND2.
+    repeat split; auto; repeat intro; specialize (H0 a); firstorder.
+Qed.
+
+Lemma PSemAction_inline_In (f : DefMethT) o:
+  forall {retK2} a calls1 calls2 readRegs newRegs (retV2 : type retK2),
+    PSemAction o a readRegs newRegs (calls1++calls2) retV2 ->
+    ~In (fst f) (map fst calls2) ->
+    forall readRegs' newRegs' calls',
+      DisjKey newRegs' newRegs ->
+      (* (forall x, ~In x calls' \/ ~In x calls2) -> *)
+      PSemAction_meth_collector f o readRegs' newRegs' calls' calls1 ->      
+      PSemAction o (inlineSingle f a) (readRegs' ++ readRegs) (newRegs' ++ newRegs) (calls'++calls2) retV2.
+Proof.
+  induction a; intros.
+  - simpl; destruct string_dec;[destruct Signature_dec|]; subst.
+    + (* specialize (PSemAction_NoDup_Calls H0) as HPsa_nd_C. *)
+      inv H0; EqDep_subst.
+      assert (In (fst f, existT SignT (projT1 (snd f)) (evalExpr e, mret)) calls1);
+        [case (in_app_or _ _ _ (Permutation_in _ (Permutation_sym (HAcalls)) (in_eq _ _))); auto; intros TMP;apply (in_map fst) in TMP; contradiction|].
+      specialize (Produce_action_from_collector _ H0 H3) as TMP; destruct TMP as [creads1 [creads2 [cupds1 [cupds2 [ccalls1 [ccalls2 [ccalls'' [cargV [cretV decomp]]]]]]]]].
+      destruct decomp as [HDisju12 [HNr21 [HC21 [HRr21 [Hceq [HC1 [HSa HSac]]]]]]].
+      inv Hceq; EqDep_subst.
+      econstructor.
+      * rewrite HNr21 in H2.
+        assert (DisjKey cupds2 (cupds1++newRegs)) as HDjk21n;[|apply HDjk21n].
+        intro; specialize (H2 k); specialize (HDisju12 k); rewrite map_app,in_app_iff, DeM1 in *.
+        clear - H2 HDisju12; firstorder fail.
+      (* * assert (forall x, ~In x ccalls2 \/ ~In x (ccalls1++calls2)) as HDj221;[|apply HDj221]. *)
+      (*   intros x; specialize (H3 x); specialize (NoDup_app_Disj MethT_dec _ _ HPsa_nd_C x) as HNd_a_d; specialize (HDisjc1' x); specialize (HDisjc12 x). *)
+      (*   rewrite HC21 in HDisjc1', H3; rewrite in_app_iff, DeM2 in *. *)
+      (*   clear - HDisjc1' HNd_a_d H3 HDisjc12; firstorder fail. *)
+      * econstructor; eauto.
+      * rewrite HRr21, <-app_assoc.
+        apply Permutation_app_head.
+        reflexivity.
+      * rewrite HNr21, <-app_assoc; reflexivity.
+      * rewrite HC21, <-app_assoc; reflexivity.
+      * eapply H; auto.
+        -- rewrite HC1 in HAcalls; simpl in *.
+           apply Permutation_cons_inv in HAcalls.
+           symmetry in HAcalls.
+           apply (PSemAction_rewrite_calls HAcalls HPSemAction).
+        -- rewrite HNr21 in H2.
+           intro; specialize (H2 k); rewrite map_app, in_app_iff in *.
+           clear - H2; firstorder fail.
+        (* -- intro x; specialize (H3 x); rewrite HC21, in_app_iff in H3. *)
+        (*    clear - H3; firstorder fail. *)
+        -- assumption.
+    + inv H0; EqDep_subst.
+      specialize (Permutation_in _ (Permutation_sym HAcalls) (in_eq _ _)); rewrite in_app_iff; intro TMP.
+      destruct TMP as [H0|H0];[|apply (in_map fst) in H0; contradiction].
+      specialize (collector_correct_snd _ H0 H3) as TMP; dest; simpl in *.
+      inv H4; EqDep_subst.
+      apply False_ind; apply n; reflexivity.
+    + inv H0; EqDep_subst.
+      specialize (Permutation_in _ (Permutation_sym HAcalls) (in_eq _ _)); intro TMP.
+      rewrite in_app_iff in TMP; destruct TMP as [H0|H0];[apply (collector_correct_fst _ H0) in H3; symmetry in H3; contradiction|].
+      apply in_split in H0; dest.
+      rewrite H0, <-Permutation_middle, Permutation_app_comm in HAcalls; simpl in *.
+      apply Permutation_cons_inv in HAcalls.
+      rewrite Permutation_app_comm in HAcalls.
+      (* assert (~In (meth, existT _ s (evalExpr e, mret)) (calls'++x++x0)); *)
+      (*   [rewrite in_app_iff; specialize (H3 (meth, existT _ s (evalExpr e, mret))); destruct H3; split; auto; *)
+      (*    apply False_ind; rewrite H0 in H3; apply H3; rewrite in_app_iff; simpl; right; left; reflexivity|]. *)
+      econstructor.
+      (* * apply H7. *)
+      * rewrite H0, app_assoc,Permutation_app_comm; simpl.
+        apply perm_skip.
+        setoid_rewrite Permutation_app_comm.
+        rewrite <-app_assoc.
+        reflexivity.
+      * eapply H; auto.
+        -- apply (PSemAction_rewrite_calls (Permutation_sym HAcalls) HPSemAction).
+        -- rewrite H0 in H1.
+           rewrite map_app, in_app_iff in *.
+           simpl in *; repeat rewrite DeM1 in *; clear - H1; firstorder fail.
+        (* -- intro x1; specialize (H3 x1). *)
+        (*    rewrite H0, <-Permutation_middle in H3. *)
+        (*    simpl in *; rewrite DeM2 in *. *)
+        (*    clear - H3; firstorder fail. *)
+        -- assumption.
+  - inv H0; EqDep_subst.
+    econstructor 2; eauto.
+  - inv H0; EqDep_subst.
+    specialize (Permutation_filter (called_by f) HUCalls) as HC1.
+    rewrite filter_app, (collector_called_by_filter_irrel H3), notIn_filter_nil, app_nil_r in HC1; auto.
+    specialize (Permutation_filter (complement (called_by f)) HUCalls) as HC2.
+    rewrite filter_app, (collector_complement_called_by_filter_nil H3), (notIn_complement_filter_irrel) in HC2; auto; simpl in *.
+    rewrite filter_app in *.
+    rewrite HC1 in H3.
+    specialize (collector_split _ _ H3) as TMP; destruct TMP as [sreads1 [sreads2 [supds1 [supds2 [scalls1 [scalls2 TMP]]]]]].
+    destruct TMP as [HRr12 [HNr12 [HC12 [HCol1 HCol2]]]].
+    econstructor 3.
+    + rewrite HNr12, HUNewRegs in H2.
+      specialize (collector_NoDupRegs1 H3); rewrite HNr12, map_app; intros TMP.
+      assert (DisjKey (supds1++newRegs0) (supds2++newRegsCont));[|apply H0].
+      intro; specialize (H2 k0); specialize (HDisjRegs k0);specialize (NoDup_app_Disj string_dec _ _ TMP k0) as TMP2.
+      repeat rewrite map_app, in_app_iff in *.
+      clear - H2 HDisjRegs TMP2; firstorder fail.
+    (* + assert (forall x, ~In x (scalls1++(filter (complement (called_by f)) calls)) \/ ~In x (scalls2++(filter (complement (called_by f)) callsCont)));[admit|]. *)
+    (*   intro x; specialize (H3 x). *)
+    (*   specialize (HDisjCalls x). *)
+    (*   specialize (collector_NoDupCalls2 H4); rewrite HC12; intro HNds12. *)
+    (*   specialize (NoDup_app_Disj MethT_dec _ _ HNds12 x) as Hdisjs12. *)
+    (*   rewrite (separate_calls_by_filter calls (called_by f)), (separate_calls_by_filter callsCont (called_by f)) in HDisjCalls. *)
+    (*   rewrite HC12, HC2 in H3. *)
+    (*   repeat rewrite in_app_iff, DeM2 in *. *)
+    (*   clear -  HDisjCalls H3 Hdisjs12. *)
+    (*   firstorder fail. *)
+    + eapply IHa.
+      * apply (PSemAction_rewrite_calls (separate_calls_by_filter calls (called_by f))) in HPSemAction.
+        apply HPSemAction.
+      * intro; apply H1; rewrite HC2, map_app, in_app_iff; left; assumption.
+      *rewrite HNr12, HUNewRegs in H2.
+       intro; specialize (H2 k0); repeat rewrite map_app, in_app_iff in *.
+       clear - H2; firstorder fail.
+      (* * intros x; specialize (H3 x). *)
+      (*   rewrite HC12, HC2 in H3. *)
+      (*   repeat rewrite in_app_iff, DeM2 in *. *)
+      (*   clear - H3; firstorder fail. *)
+      * apply HCol1.
+    + rewrite HRr12, HUReadRegs.
+      repeat rewrite <-app_assoc.
+      apply Permutation_app_head.
+      rewrite app_assoc,Permutation_app_comm.
+      rewrite app_assoc.
+      rewrite Permutation_app_comm.
+      apply Permutation_app_head.
+      apply Permutation_app_comm.
+    + rewrite HNr12, HUNewRegs.
+      repeat rewrite <-app_assoc.
+      apply Permutation_app_head.
+      repeat rewrite app_assoc.
+      apply Permutation_app_tail.
+      apply Permutation_app_comm.
+    + rewrite HC2, HC12.
+      repeat rewrite <-app_assoc.
+      apply Permutation_app_head.
+      rewrite app_assoc, Permutation_app_comm.
+      rewrite app_assoc.
+      rewrite Permutation_app_comm; apply Permutation_app_head.
+      apply Permutation_app_comm.
+    + eapply H; eauto.
+      * apply (PSemAction_rewrite_calls (separate_calls_by_filter callsCont (called_by f)) HPSemActionCont).
+      * rewrite HC2, map_app,in_app_iff in H1; dest; clear - H1; tauto.
+      * rewrite HNr12, HUNewRegs in H2.
+        intro k0; specialize (H2 k0).
+        repeat rewrite map_app, in_app_iff in H2.
+        clear - H2; firstorder fail.
+      (* * intro x; specialize (H3 x). *)
+      (*   rewrite HC12, HC2 in H3. *)
+      (*   repeat rewrite in_app_iff, DeM2 in H3. *)
+      (*   clear - H3; firstorder fail. *)
+  - inv H0; EqDep_subst.
+    simpl; econstructor 4; eauto.
+  - inv H0; EqDep_subst.
+    simpl; econstructor 5.
+    + apply HRegVal.
+    + eapply H; eauto.
+    + rewrite HNewReads.
+      symmetry.
+      apply Permutation_middle.
+  - inv H; EqDep_subst.
+    simpl; econstructor 6; auto.
+    + assert (key_not_In r (newRegs'++newRegs0));[|apply H].
+      intro; rewrite in_app_iff.
+      specialize (HDisjRegs v).
+      intro; destruct H; auto.
+      apply (in_map fst) in H; simpl in *.
+      rewrite HANewRegs in H1; specialize (H1 r).
+      destruct H1;[contradiction|apply H1; left; reflexivity].
+    + rewrite HANewRegs.
+      rewrite Permutation_app_comm; simpl.
+      apply perm_skip, Permutation_app_comm.
+    + eapply IHa; eauto.
+      rewrite HANewRegs in H1; intro k0; specialize (H1 k0); simpl in *.
+      clear - H1; firstorder fail.
+  - inv H0; EqDep_subst; simpl.
+    + specialize (Permutation_filter (called_by f) HUCalls) as HC1.
+      rewrite filter_app, (collector_called_by_filter_irrel H3), notIn_filter_nil, app_nil_r in HC1; auto.
+      specialize (Permutation_filter (complement (called_by f)) HUCalls) as HC2.
+      rewrite filter_app, (collector_complement_called_by_filter_nil H3), (notIn_complement_filter_irrel) in HC2; auto; simpl in *.
+      rewrite filter_app in *.
+      rewrite HC1 in H3.
+      specialize (collector_split _ _ H3) as TMP; destruct TMP as [sreads1 [sreads2 [supds1 [supds2 [scalls1 [scalls2 TMP]]]]]].
+      destruct TMP as [HRr12 [HNr12 [HC12 [HCol1 HCol2]]]].
+      econstructor 7.
+      * rewrite HNr12, HUNewRegs in H2.
+        specialize (collector_NoDupRegs1 H3); rewrite HNr12, map_app; intros TMP.
+        assert (DisjKey (supds1++newRegs1) (supds2++newRegs2));[|apply H0].
+        intro; specialize (H2 k0); specialize (HDisjRegs k0);specialize (NoDup_app_Disj string_dec _ _ TMP k0) as TMP2.
+        repeat rewrite map_app, in_app_iff in *.
+        clear - H2 HDisjRegs TMP2; firstorder fail.
+      (* * assert (forall x, ~In x (scalls1++(filter (complement (called_by f)) calls0)) \/ ~In x (scalls2++(filter (complement (called_by f)) calls3)));[|apply H0]. *)
+      (*   intro x; specialize (H3 x). *)
+      (*   specialize (HDisjCalls x). *)
+      (*   specialize (collector_NoDupCalls2 H4); rewrite HC12; intro HNds12. *)
+      (*   specialize (NoDup_app_Disj MethT_dec _ _ HNds12 x) as Hdisjs12. *)
+      (*   rewrite (separate_calls_by_filter calls0 (called_by f)), (separate_calls_by_filter calls3 (called_by f)) in HDisjCalls. *)
+      (*   rewrite HC12, HC2 in H3. *)
+      (*   repeat rewrite in_app_iff, DeM2 in *. *)
+      (*   clear -  HDisjCalls H3 Hdisjs12. *)
+      (*   firstorder fail. *)
+      * assumption.
+      * eapply IHa1.
+        -- apply (PSemAction_rewrite_calls (separate_calls_by_filter calls0 (called_by f))) in HAction.
+           apply HAction.
+        -- intro; apply H1; rewrite HC2, map_app, in_app_iff; left; assumption.
+        -- rewrite HNr12, HUNewRegs in H2.
+           intro; specialize (H2 k0); repeat rewrite map_app, in_app_iff in *.
+           clear - H2; firstorder fail.
+        (* -- intros x; specialize (H3 x). *)
+        (*    rewrite HC12, HC2 in H3. *)
+        (*    repeat rewrite in_app_iff, DeM2 in *. *)
+        (*    clear - H3; firstorder fail. *)
+        -- apply HCol1.
+      * eapply H.
+        -- apply (PSemAction_rewrite_calls (separate_calls_by_filter calls3 (called_by f)) HPSemAction).
+        -- rewrite HC2, map_app,in_app_iff in H1; clear -H1; firstorder fail.
+        -- rewrite HNr12, HUNewRegs in H2.
+           intro k0; specialize (H2 k0).
+           repeat rewrite map_app, in_app_iff in H2.
+           clear - H2; firstorder fail.
+        (* -- intro x; specialize (H3 x). *)
+        (*    rewrite HC12, HC2 in H3. *)
+        (*    repeat rewrite in_app_iff, DeM2 in H3. *)
+        (*    clear - H3; firstorder fail. *)
+        --apply HCol2.
+      * rewrite HRr12, HUReadRegs.
+        repeat rewrite <-app_assoc.
+        apply Permutation_app_head.
+        rewrite app_assoc,Permutation_app_comm.
+        rewrite app_assoc.
+        rewrite Permutation_app_comm.
+        apply Permutation_app_head.
+        apply Permutation_app_comm.
+      * rewrite HNr12, HUNewRegs.
+        repeat rewrite <-app_assoc.
+        apply Permutation_app_head.
+        repeat rewrite app_assoc.
+        apply Permutation_app_tail.
+        apply Permutation_app_comm.
+      * rewrite HC2, HC12.
+        repeat rewrite <-app_assoc.
+        apply Permutation_app_head.
+        repeat rewrite app_assoc.
+        apply Permutation_app_tail.
+        apply Permutation_app_comm.
+    + specialize (Permutation_filter (called_by f) HUCalls) as HC1.
+      rewrite filter_app, (collector_called_by_filter_irrel H3), notIn_filter_nil, app_nil_r in HC1; auto.
+      specialize (Permutation_filter (complement (called_by f)) HUCalls) as HC2.
+      rewrite filter_app, (collector_complement_called_by_filter_nil H3), (notIn_complement_filter_irrel) in HC2; auto; simpl in *.
+      rewrite filter_app in *.
+      rewrite HC1 in H3.
+      specialize (collector_split _ _ H3) as TMP; destruct TMP as [sreads1 [sreads2 [supds1 [supds2 [scalls1 [scalls2 TMP]]]]]].
+      destruct TMP as [HRr12 [HNr12 [HC12 [HCol1 HCol2]]]].
+      econstructor 8.
+      * rewrite HNr12, HUNewRegs in H2.
+        specialize (collector_NoDupRegs1 H3); rewrite HNr12, map_app; intros TMP.
+        assert (DisjKey (supds1++newRegs1) (supds2++newRegs2));[|apply H0].
+        intro; specialize (H2 k0); specialize (HDisjRegs k0);specialize (NoDup_app_Disj string_dec _ _ TMP k0) as TMP2.
+        repeat rewrite map_app, in_app_iff in *.
+        clear - H2 HDisjRegs TMP2; firstorder fail.
+      (* * assert (forall x, ~In x (scalls1++(filter (complement (called_by f)) calls0)) \/ ~In x (scalls2++(filter (complement (called_by f)) calls3)));[|apply H0]. *)
+      (*   intro x; specialize (H3 x). *)
+      (*   specialize (HDisjCalls x). *)
+      (*   specialize (collector_NoDupCalls2 H4); rewrite HC12; intro HNds12. *)
+      (*   specialize (NoDup_app_Disj MethT_dec _ _ HNds12 x) as Hdisjs12. *)
+      (*   rewrite (separate_calls_by_filter calls0 (called_by f)), (separate_calls_by_filter calls3 (called_by f)) in HDisjCalls. *)
+      (*   rewrite HC12, HC2 in H3. *)
+      (*   repeat rewrite in_app_iff, DeM2 in *. *)
+      (*   clear -  HDisjCalls H3 Hdisjs12. *)
+      (*   firstorder fail. *)
+      * assumption.
+      * eapply IHa2.
+        -- apply (PSemAction_rewrite_calls (separate_calls_by_filter calls0 (called_by f))) in HAction.
+           apply HAction.
+        -- intro; apply H1; rewrite HC2, map_app, in_app_iff; left; assumption.
+        -- rewrite HNr12, HUNewRegs in H2.
+           intro; specialize (H2 k0); repeat rewrite map_app, in_app_iff in *.
+           clear - H2; firstorder fail.
+        (* -- intros x; specialize (H3 x). *)
+        (*    rewrite HC12, HC2 in H3. *)
+        (*    repeat rewrite in_app_iff, DeM2 in *. *)
+        (*    clear - H3; firstorder fail. *)
+        -- apply HCol1.
+      * eapply H.
+        -- apply (PSemAction_rewrite_calls (separate_calls_by_filter calls3 (called_by f)) HPSemAction).
+        -- rewrite HC2, map_app,in_app_iff in H1; dest; clear -H1; firstorder fail.
+        -- rewrite HNr12, HUNewRegs in H2.
+           intro k0; specialize (H2 k0).
+           repeat rewrite map_app, in_app_iff in H2.
+           clear - H2; firstorder fail.
+        (* -- intro x; specialize (H3 x). *)
+        (*    rewrite HC12, HC2 in H3. *)
+        (*    repeat rewrite in_app_iff, DeM2 in H3. *)
+        (*    clear - H3; firstorder fail. *)
+        --apply HCol2.
+      * rewrite HRr12, HUReadRegs.
+        repeat rewrite <-app_assoc.
+        apply Permutation_app_head.
+        rewrite app_assoc,Permutation_app_comm.
+        rewrite app_assoc.
+        rewrite Permutation_app_comm.
+        apply Permutation_app_head.
+        apply Permutation_app_comm.
+      * rewrite HNr12, HUNewRegs.
+        repeat rewrite <-app_assoc.
+        apply Permutation_app_head.
+        repeat rewrite app_assoc.
+        apply Permutation_app_tail.
+        apply Permutation_app_comm.
+      * rewrite HC2, HC12.
+        repeat rewrite <-app_assoc.
+        apply Permutation_app_head.
+        repeat rewrite app_assoc.
+        apply Permutation_app_tail.
+        apply Permutation_app_comm.
+  - inv H; EqDep_subst.
+    econstructor 9; eauto.
+  - inv H; EqDep_subst.
+    econstructor 10; eauto.
+  - inv H; EqDep_subst.
+    apply app_eq_nil in HCalls; dest; subst.
+    inv H2; simpl in *.
+    + econstructor 11; eauto.
+    + apply Permutation_nil in H7; discriminate.
+Qed.  
+
+Lemma PPlusSubsteps_inline_notIn f m o upds execs calls:
+  PPlusSubsteps m o upds execs calls ->
+  ~In (fst f) (map fst calls) ->
+  PPlusSubsteps (inlinesingle_BaseModule m f) o upds execs calls.
+Proof.
+  induction 1; simpl; intros.
+  - econstructor 1; eauto.
+  - rewrite HUpds, HExecs, HCalls.
+    apply (in_map (inlinesingle_Rule f)) in HInRules.
+    econstructor 2 with (u := u) (reads := reads); eauto.
+    + eapply PSemAction_inline_notIn; eauto.
+      intro; apply H0; rewrite HCalls, map_app, in_app_iff; left; assumption.
+    + eapply IHPPlusSubsteps.
+      intro; apply H0; rewrite HCalls, map_app, in_app_iff; right; assumption.
+  - rewrite HUpds, HExecs, HCalls.
+    apply (in_map (inlinesingle_Meth f)) in HInMeths; destruct fb.
+    econstructor 3 with (u := u) (reads := reads); simpl; eauto.
+    + simpl; eapply PSemAction_inline_notIn; eauto.
+      intro; apply H0; rewrite HCalls, map_app, in_app_iff; left; assumption.
+    + eapply IHPPlusSubsteps.
+      intro; apply H0; rewrite HCalls, map_app, in_app_iff; right; assumption.
+Qed.
+
+Lemma KeyMatching2 (l : list DefMethT) (a b : DefMethT):
+  NoDup (map fst l) -> In a l -> In b l -> fst a = fst b -> a = b.
+Proof.
+  induction l; intros.
+  - inv H0.
+  - destruct H0, H1; subst; auto; simpl in *.
+    + inv H.
+      apply False_ind, H4.
+      rewrite H2, in_map_iff.
+      exists b; firstorder.
+    + inv H.
+      apply False_ind, H4.
+      rewrite <- H2, in_map_iff.
+      exists a; firstorder.
+    + inv H.
+      eapply IHl; eauto.
+Qed.
+
+Lemma Substeps_permutation_invariant m o l l' :
+  l [=] l' ->
+  Substeps m o l ->
+  Substeps m o l'.
+Proof.
+  induction 1; intros; auto.
+  - inv H0.
+    + inv HLabel.
+      econstructor 2; eauto; setoid_rewrite <- H; auto.
+    + inv HLabel.
+      econstructor 3; eauto; setoid_rewrite <- H; auto.
+  - inv H.
+    + inv HLabel.
+      inv HSubstep; inv HLabel.
+      * specialize (HNoRle _ (in_eq _ _)); simpl in *; contradiction.
+      * econstructor 3; eauto; intros.
+        -- destruct H; subst.
+           ++ simpl.
+              specialize (HDisjRegs _ (in_eq _ _)); simpl in *.
+              apply DisjKey_Commutative; assumption.
+           ++ eapply HDisjRegs0; auto.
+        (* -- destruct H0; dest; destruct H0; subst; simpl in *. *)
+        (*    ++ eapply HNoCall; eauto. *)
+        (*       exists (u0, (Meth (fn, existT SignT (projT1 fb) (argV, retV)), cs0)); split; *)
+        (*         [left; reflexivity|auto]. *)
+        (*    ++ eapply HNoCall0; eauto. *)
+        (*       exists x; firstorder. *)
+        (* -- unfold InExec in *; simpl in *. *)
+        (*    destruct H;[discriminate|auto]. *)
+        -- econstructor 2; eauto; intros.
+           ++ eapply HDisjRegs; right; assumption.
+           ++ eapply HNoRle; right; assumption.
+           (* ++ eapply HNoCall; eauto. *)
+           (*    destruct H0; dest. *)
+           (*    exists x; split; auto; right; assumption. *)
+    + inv HLabel.
+      inv HSubsteps; inv HLabel.
+      * econstructor 2; eauto; intros.
+        -- destruct H; subst.
+           ++ simpl.
+              specialize (HDisjRegs _ (in_eq _ _)); simpl in *.
+              apply DisjKey_Commutative; assumption.
+           ++ eapply HDisjRegs0; auto.
+        -- destruct H; subst; simpl in *; auto.
+           eapply HNoRle; eauto.
+        (* -- destruct H0; dest; destruct H0; subst; simpl in *. *)
+        (*    ++ eapply HNoCall; eauto. *)
+        (*       exists (u0, (Rle rn, cs0)); split; auto; left; reflexivity. *)
+        (*    ++ eapply HNoCall0; eauto. *)
+        (*       exists x; firstorder. *)
+        -- econstructor 3; eauto; intros.
+           ++ eapply HDisjRegs; right; assumption.
+           (* ++ eapply HNoCall; eauto. *)
+           (*    destruct H0; dest. *)
+           (*    exists x; split; auto; right; assumption. *)
+           (* ++ unfold InExec in *; simpl in *. *)
+           (*    eapply HNoExec; right; assumption. *)
+      * econstructor 3; eauto; intros.
+        -- destruct H; subst; simpl.
+           ++ specialize (HDisjRegs _ (in_eq _ _)); simpl in *.
+              apply DisjKey_Commutative; assumption.
+           ++ eapply HDisjRegs0; eauto.
+        (* -- destruct H0; dest; destruct H0; subst; simpl in *. *)
+        (*    ++ eapply HNoCall; eauto. *)
+        (*       exists (u0, (Meth (fn0, existT SignT (projT1 fb0) (argV0, retV0)), cs0)); *)
+        (*         split; auto;left; reflexivity. *)
+        (*    ++ eapply HNoCall0; eauto. *)
+        (*       exists x; split; auto. *)
+        (* -- unfold InExec in *; simpl in *. *)
+        (*    destruct H. *)
+        (*    ++ inv H; EqDep_subst. *)
+        (*       destruct fb, fb0; simpl in *; subst; EqDep_subst. *)
+        (*       apply HNoExec; left; reflexivity. *)
+        (*    ++ apply HNoExec0; auto. *)
+        -- econstructor 3; auto; auto;[apply HAction | | ]; auto; intros.
+           ++ eapply HDisjRegs; right; assumption.
+           (* ++ eapply HNoCall; eauto. *)
+           (*    destruct H0; dest. *)
+           (*    exists x; split; auto; right; assumption. *)
+           (* ++ unfold InExec in *; simpl in *. *)
+           (*    apply HNoExec; right; assumption. *)
+Qed.
+
+Lemma extract_exec (f : DefMethT) m o l u cs fb:
+  NoDup (map fst (getMethods m)) ->
+  In f (getMethods m) ->
+  Substeps m o ((u, (Meth ((fst f), fb), cs))::l) ->
+  exists reads e mret,
+    fb =  existT SignT (projT1 (snd f)) (e, mret) /\
+    DisjKey u (getLabelUpds l) /\
+    (* DisjKey cs (getLabelCalls l) /\ *)
+    SemAction o ((projT2 (snd f) type) e) reads u cs mret /\
+    Substeps m o l.
+Proof.
+  intros.
+  inv H1.
+  - inv HLabel.
+  - inv HLabel.
+    destruct f, s0, fb0; simpl in *; subst;EqDep_subst.
+    specialize (KeyMatching2 _ _ _ H HInMeths H0 (eq_refl)) as TMP.
+    inv TMP; EqDep_subst.
+    exists reads, argV, retV; repeat split; auto.
+    + apply DisjKey_Commutative.
+      clear - HDisjRegs.
+      induction ls.
+      * intro; left; auto.
+      * unfold getLabelUpds in *; simpl.
+        intro; rewrite map_app, in_app_iff, DeM1.
+        specialize (HDisjRegs a (in_eq _ _) k) as TMP; simpl in *.
+        assert (forall x, In x ls -> DisjKey (fst x) u0);[intros; eapply HDisjRegs; eauto|].
+        specialize (IHls H k) as TMP2; destruct TMP, TMP2; firstorder fail.
+Qed.
+
+Lemma List_FullLabel_perm_getLabelUpds_perm l1 l2:
+  List_FullLabel_perm l1 l2 ->
+  getLabelUpds l1 [=] getLabelUpds l2.
+Proof.
+  induction 1.
+  - reflexivity.
+  - unfold getLabelUpds in *; inv H; simpl in *.
+    rewrite H1, IHList_FullLabel_perm; reflexivity.
+  - unfold getLabelUpds in *; inv H; inv H0; simpl in *.
+    rewrite H2, H, IHList_FullLabel_perm; repeat rewrite app_assoc.
+    apply Permutation_app_tail.
+    apply Permutation_app_comm.
+  - rewrite IHList_FullLabel_perm1, IHList_FullLabel_perm2; reflexivity.
+Qed.
+
+Lemma List_FullLabel_perm_getLabelCalls_perm l1 l2:
+  List_FullLabel_perm l1 l2 ->
+  getLabelCalls l1 [=] getLabelCalls l2.
+Proof.
+  induction 1.
+  - reflexivity.
+  - unfold getLabelCalls in *; inv H; simpl in *.
+    rewrite H3, IHList_FullLabel_perm; reflexivity.
+  - unfold getLabelCalls in *; inv H; inv H0; simpl in *.
+    rewrite H4, H5, IHList_FullLabel_perm; repeat rewrite app_assoc.
+    apply Permutation_app_tail.
+    apply Permutation_app_comm.
+  - rewrite IHList_FullLabel_perm1, IHList_FullLabel_perm2; reflexivity.
+Qed.
+
+Lemma List_FullLabel_perm_getLabelExecs_perm l1 l2:
+  List_FullLabel_perm l1 l2 ->
+  getLabelExecs l1 [=] getLabelExecs l2.
+Proof.
+  induction 1.
+  - reflexivity.
+  - unfold getLabelExecs in *; inv H; simpl in *.
+    rewrite IHList_FullLabel_perm; reflexivity.
+  - unfold getLabelExecs in *; inv H; inv H0; simpl in *.
+    rewrite IHList_FullLabel_perm.
+    apply perm_swap.
+  - rewrite IHList_FullLabel_perm1, IHList_FullLabel_perm2; reflexivity.
+Qed.
+
+Lemma extract_exec_P (f : DefMethT) m o l u cs fb:
+  NoDup (map fst (getMethods m)) ->
+  In f (getMethods m) ->
+  PSubsteps m o ((u, (Meth ((fst f),fb), cs))::l) ->
+  exists reads e mret,
+    fb = existT SignT (projT1 (snd f)) (e, mret) /\
+    DisjKey u (getLabelUpds l) /\
+    PSemAction o ((projT2 (snd f) type) e) reads u cs mret /\
+    PSubsteps m o l.
+Proof.
+  intros.
+  apply (PSubsteps_Substeps) in H1; dest.
+  specialize (List_FullLabel_perm_in H2 _ (in_eq _ _)) as TMP; dest.
+  specialize (in_split _ _ H6) as TMP; dest.
+  rewrite H7, <- Permutation_middle in H2.
+  specialize (List_FullLabel_perm_cons_inv H5 H2) as P2.
+  inv H5.
+  apply (Substeps_permutation_invariant (Permutation_sym (Permutation_middle _ _ _))) in H4.
+  apply (extract_exec f) in H4; auto; dest.
+  exists x0, x1, x4; repeat split; auto.
+  + rewrite H11.
+    rewrite (List_FullLabel_perm_getLabelUpds_perm P2).
+    assumption.
+  (* + rewrite H14. *)
+  (*   rewrite (List_FullLabel_perm_getLabelCalls_perm P2). *)
+  (*   assumption. *)
+  + symmetry in H1, H11, H14.
+    apply (PSemAction_rewrite_state H1).
+    apply (PSemAction_rewrite_newRegs H11).
+    apply (PSemAction_rewrite_calls H14).
+    apply SemAction_PSemAction; assumption.
+  + rewrite P2, H1.
+    apply Substeps_PSubsteps; assumption.
+Qed.
+
+Corollary extract_exec_PPlus (f : DefMethT) m o upds execs calls fb:
+  NoDup (map fst (getMethods m)) ->
+  In f (getMethods m) ->
+  PPlusSubsteps m o upds ((Meth ((fst f),fb))::execs) calls ->
+  exists reads upds1 upds2 calls1 calls2 e mret,
+    fb = existT SignT (projT1 (snd f)) (e, mret) /\
+    PSemAction o ((projT2 (snd f) type) e) reads upds1 calls1 mret /\
+    upds [=] upds1++upds2 /\
+    calls [=] calls1++calls2 /\
+    DisjKey upds1 upds2 /\
+    (* DisjKey calls1 calls2 /\ *)
+    PPlusSubsteps m o upds2 execs calls2.
+Proof.
+  intros.
+  apply (PPlusSubsteps_PSubsteps) in H1; dest.
+  unfold getLabelExecs, getLabelUpds, getLabelCalls in *.
+  specialize (Permutation_in _ H3 (in_eq _ _)) as H3'.
+  rewrite (in_map_iff) in H3'; dest; destruct x0, p.
+  apply in_split in H6; dest; rewrite H6,map_app in H4, H3, H2;rewrite concat_app in *; simpl in *.
+  rewrite H5 in *;rewrite H6, <-Permutation_middle in H1.
+  rewrite <- Permutation_middle, <- map_app in H3.
+  apply Permutation_cons_inv in H3.
+  apply extract_exec_P in H1; eauto; dest.
+  exists x2, r, (getLabelUpds (x0++x1)), m0, (getLabelCalls (x0++x1)), x3, x4; repeat split; auto;
+    [rewrite H2; unfold getLabelUpds| rewrite H4; unfold getLabelCalls | rewrite H3; apply PSubsteps_PPlusSubsteps; assumption];
+    rewrite map_app, concat_app; repeat rewrite app_assoc; apply Permutation_app_tail; rewrite Permutation_app_comm; reflexivity.
+Qed.
+
+Lemma rewrite_called_execs:
+  forall calls execs,
+    (forall f, getNumFromCalls f calls <= getNumFromExecs f execs)%Z ->
+    exists execs',
+      execs [=] ((map Meth (calls))++execs').
+Proof.
+  induction calls; intros.
+  - exists execs; reflexivity.
+  - specialize (H a) as P1.
+    rewrite getNumFromCalls_eq_cons in P1; auto.
+    assert (getNumFromCalls a calls <= getNumFromExecs a execs)%Z;[Omega.omega|].
+    specialize (IHcalls H0).
+    simpl in P1; destruct (MethT_dec a a);[|apply False_ind, n; reflexivity].
+    
+    
+    (forall f, In f calls -> In (Meth f) execs) ->
+    NoDup execs ->
+    NoDup calls ->
+    (filter (called_execs calls) execs) [=] (map Meth calls).
+Proof.
+  induction calls; intros.
+  - unfold called_execs; simpl.
+    assert ((fun x => match x with |Rle _ | _ => false end) = (fun _ => false));[
+      apply functional_extensionality; destruct x; reflexivity|].
+    rewrite H2; rewrite filter_false; reflexivity.
+  - unfold called_execs in *; simpl in *.
+    specialize (H a (or_introl _ eq_refl)) as H'.
+    apply in_split in H'; dest; rewrite H2,<-Permutation_middle.
+    simpl; unfold methcmp; destruct MethT_dec;[simpl|apply False_ind; apply n; reflexivity].
+    apply Permutation_cons;[reflexivity|].
+    assert (~In (Meth a) (x++x0)).
+    + rewrite H2 in H0; rewrite <- Permutation_middle in H0.
+      inv H0; assumption.
+    + specialize (reduce_called_execs_list _ _ H3 calls) as TMP.
+      unfold called_execs, methcmp in *; simpl in *.
+      rewrite TMP.
+      eapply IHcalls.
+      * intros.
+        rewrite H2 in H; specialize (H _ (or_intror _ H4)).
+        rewrite <- Permutation_middle in H.
+        destruct H;[inv H; inv H1; contradiction| assumption].
+      * rewrite H2, <-Permutation_middle in H0; inv H0; assumption.
+      * inv H1; assumption.
+Qed.
+
+Lemma MatchingExecCalls_flat_surjective f calls execs m :
+  In f (getMethods m) ->
+  MatchingExecCalls_flat calls execs m ->
+  forall g,
+    In g (filter (called_by f) calls) -> In (Meth g) execs.
+Proof.
+  unfold MatchingExecCalls_flat.
+  induction calls; intros.
+  - contradiction.
+  - unfold called_by in H1; simpl in *.
+    destruct string_dec; subst; simpl in *.
+    + destruct H1; subst.
+      * apply (in_map fst) in H; rewrite e in H.
+        apply (H0 _ (or_introl _ (eq_refl)) H).
+      * eapply IHcalls; eauto.
+    + eapply IHcalls;eauto.
+Qed.
+
+Lemma filter_preserves_NoDup A (f : A -> bool) l :
+  NoDup l ->
+  NoDup (filter f l).
+Proof.
+  induction 1.
+  - simpl; constructor.
+  - unfold filter; destruct (f x); fold (filter f l); auto.
+    + econstructor; eauto.
+      intro; apply H.
+      rewrite filter_In in H1; dest; assumption.
+Qed.
+
+Lemma PPlusSubsteps_inline_In f m o upds execs calls :
+  NoDup (map fst (getMethods m)) ->
+  In f (getMethods m) ->
+  MatchingExecCalls_flat calls execs m ->
+  PPlusSubsteps m o upds execs calls ->
+  PPlusSubsteps (inlinesingle_BaseModule m f) o upds (filter (complement (called_execs (filter (called_by f) calls))) execs) (filter (complement (called_by f)) calls).
+Proof.
+  induction 4; simpl.
+  - econstructor 1; auto.
+  - rewrite HUpds, HExecs, HCalls; simpl.
+    rewrite filter_app.
+    destruct (in_dec string_dec (fst f) (map fst cs)).
+    + specialize (fst_produce_snd _ _ i) as TMP; dest.
+      unfold MatchingExecCalls_flat in H1; setoid_rewrite HCalls in H1.
+      specialize (H1 _ (in_or_app _ _ _ (or_introl _ H3))) as TMP; simpl in *.
+      specialize (TMP (in_map fst _ _ H0)); simpl in *.
+      rewrite HExecs in TMP; destruct TMP;[discriminate|].
+      specialize (in_split _ _ H4) as TMP; dest.
+      rewrite H5, <- Permutation_middle in H2.
+      admit.
+    + admit.
+  - admit.
+Admitted.
+
 Lemma PSemAction_inline_In (f : DefMethT) o readRegs' newRegs' calls' argV retV1:
     PSemAction o (projT2 (snd f) type argV) readRegs' newRegs' calls' retV1 ->
     forall {retK2} a readRegs newRegs calls (retV2 : type retK2),
